clean proof

compiler/src/toEC.ml
@@ -1180,18 +1180,14 @@ let pp_prog fmt model globs funcs =
     | Normal -> () in
 
   Format.fprintf fmt 
-     "@[<v>%s.@ %s.@ @ %a%a@ %a@ %s@ %s@ module M = {@   @[<v>%a%a@]@ }.@ %s@ @]@."
+     "@[<v>%s.@ %s.@ %s.@ @ %a%a@ %a@ %s@ module M = {@   @[<v>%a%a@]@ }.@ %s@ @]@."
     "require import AllCore IntDiv CoreMap List"
     "from Jasmin require import JModel"
+    "require import Leakage_models"
     (pp_arrays "Array") env.arrsz
     (pp_arrays "WArray") env.warrsz
     (pp_list "@ @ " (pp_glob_decl env)) globs
     (* TODO: provide division leakage for all word sizes *)
-    "abstract theory ALeakageModel.
-    op leak_div_32 : W32.t -> W32.t -> address list.
-    op leak_div_64 : W64.t -> W64.t -> address list.
-    op leak_mem : address -> address.
-end ALeakageModel.\n"
     "theory T.\nclone import ALeakageModel as LeakageModel.\n"
     pp_leakages env
     (pp_list "@ @ " (pp_fun env)) funcs
