casestudy/leakage_models.ec
@@ -1,88 +1,99 @@
 require import AllCore IntDiv CoreMap List.
 from Jasmin require import JModel.
 
-(* Leakage models BL, TV, CL, and TV+CL and common lemmas for the verification of the copy-mac implementations. *)
+(* Leakage models TV, BL, TV+CL, CL                                           *) 
+(* Strongest on top                                                           *)
+(*                     TV = log2 for div + id for mem                         *)
+(*                      /                    \                                *)
+(*                     /                      \                               *)
+(*   BL = none for div + id for mem      TV + CL = log2 for div + /64 for mem *)
+(*                     \                      /                               *)
+(*                      \                    /                                *) 
+(*                    CL =  none for div + /64 for mem                        *)
 
-theory LeakageModelBL.
-op leak_mem (a: address) : address = a.
-op leak_div_32 (a b: W32.t) : address list = [].
-op leak_div_64 (a b: W64.t) : address list = [].
-end LeakageModelBL.
+abstract theory ALeakageModel.
+  op leak_div_32 : W32.t -> W32.t -> address list.
+  op leak_div_64 : W64.t -> W64.t -> address list.
+  op leak_mem : address -> address.
+end ALeakageModel.
 
-op leak_div (a: W32.t) : int =
-  lzcnt (rev (w2bits a)).
+op leak_div_none (a b : 'a) : address list = [].
 
-theory LeakageModelTV.
+theory LD32.
+  op leak_div (a:W32.t) : int = lzcnt (rev (w2bits a)).
+end LD32. export LD32.
 
-op leak_div_32 (a b: W32.t) : address list =
-[ leak_div a ; to_uint b ].
+theory LD64.
+  op leak_div (a:W64.t) : int = lzcnt (rev (w2bits a)).
+end LD64. export LD64.
 
-op leak_div_64 (a b: W64.t) : address list =
-[ to_uint a ; to_uint b ].
+op leak_div_32_TV (a b: W32.t) : address list =
+  [ leak_div a; to_uint b].
 
-op leak_mem = LeakageModelBL.leak_mem.
+op leak_div_64_TV (a b: W64.t) : address list =
+  [ leak_div a; to_uint b] .
 
-end LeakageModelTV.
+op leak_mem_id (a:address) : address = a.
+op leak_mem_CL (a:address) : address = a %/ 64.
 
-theory LeakageModelCL.
+clone ALeakageModel as LeakageModelTV with 
+  op leak_div_32 = leak_div_32_TV,
+  op leak_div_64 = leak_div_64_TV,
+  op leak_mem    = leak_mem_id.
 
-op leak_div_32 = LeakageModelBL.leak_div_32.
-op leak_div_64 = LeakageModelBL.leak_div_64.
+clone ALeakageModel as LeakageModelBL with
+  op leak_div_32 = leak_div_none,
+  op leak_div_64 = leak_div_none,
+  op leak_mem    = leak_mem_id.
 
-op leak_mem (a: address) : address =
-  a %/ 64.
+clone ALeakageModel as LeakageModelTVCL with 
+  op leak_div_32 = leak_div_32_TV,
+  op leak_div_64 = leak_div_64_TV,
+  op leak_mem    = leak_mem_CL.
 
-end LeakageModelCL.
+clone ALeakageModel as LeakageModelCL with
+  op leak_div_32 = leak_div_none,
+  op leak_div_64 = leak_div_none,
+  op leak_mem    = leak_mem_CL.
 
-theory LeakageModelTVCL.
-op leak_div_32 = LeakageModelTV.leak_div_32.
-op leak_div_64 = LeakageModelTV.leak_div_64.
-op leak_mem = LeakageModelCL.leak_mem.
-end LeakageModelTVCL.
-
+(* and common lemmas for the verification of the copy-mac implementations. *)
 lemma leak_div_or (x y : W32.t) : leak_div (x `|` y) = min (leak_div x) (leak_div y).
-    proof.
-      rewrite /leak_div /w2bits.
-      elim/natind: 32.
-      + by move=> n hn; rewrite !mkseq0_le 1..3:// /= rev_nil.
-    move=> n hn hrec; rewrite !mkseqS 1..3:// !rev_rcons /= hrec; smt(lzcnt_size).
-  qed.
+proof.
+  rewrite /leak_div /w2bits.
+  elim/natind: 32.
+  + by move=> n hn; rewrite !mkseq0_le 1..3:// /= rev_nil.
+  move=> n hn hrec; rewrite !mkseqS 1..3:// !rev_rcons /= hrec; smt(lzcnt_size).
+qed.
 
 lemma leak_div_bound (w:W32.t) : 0 <= leak_div w <= 32.
-    proof. smt (lzcnt_size size_mkseq size_rev). qed.
+proof. smt (lzcnt_size size_mkseq size_rev). qed.
+
+import StdOrder.IntOrder Ring.IntID.
 
 lemma nosmt ltr_weexpn2l x m n:
-    2 <= x => 0 <= m => 0 <= n =>
-    m < n <=> x ^ m < x ^ n.
-    proof.
-    move=> h1 h2 h3; case: (m < n) => /= h4.
-      + have -> : n = (n - m) + m by ring.
-      rewrite Ring.IntID.exprD_nneg 1:/# 1://.
-      rewrite -{1}(Ring.IntID.div1r (x^m)).
-      rewrite StdOrder.IntOrder.ltr_pmul2r.
-      + smt (StdOrder.IntOrder.expr_gt0).
-      smt (StdOrder.IntOrder.exprn_egt1).
-      have -> : m = (m - n) + n by ring.
-      rewrite Ring.IntID.exprD_nneg 1:/# 1:// -lezNgt.
-      rewrite -{1}(Ring.IntID.div1r (x^n)).
-      rewrite StdOrder.IntOrder.ler_pmul2r.
-      + smt (StdOrder.IntOrder.expr_gt0).
-      smt (StdOrder.IntOrder.exprn_ege1).
-  qed.
+  2 <= x => 0 <= m => 0 <= n =>
+  m < n <=> x ^ m < x ^ n.
+proof.
+  move=> h1 h2 h3; case: (m < n) => /= h4.
+  + have -> : n = (n - m) + m by ring.
+    by rewrite exprD_nneg 1:/# 1:// -{1}(div1r (x^m)) ltr_pmul2r; smt (expr_gt0 exprn_egt1).
+  have -> : m = (m - n) + n by ring.
+  rewrite exprD_nneg 1:/# 1:// -lezNgt -{1}(div1r (x^n)) ler_pmul2r; smt (expr_gt0 exprn_ege1).
+qed.
 
 lemma leak_div_le (w1 w2: W32.t) : to_uint w1 <= to_uint w2 => leak_div w2 <= leak_div w1.
-    proof.
-      rewrite W32.to_uintE /leak_div.
-      have := lzcnt_bound (w2bits w1).
-      have := lzcnt_bound (w2bits w2).
-      rewrite !size_w2bits => h1 h2 h3.
-      have : (if 32 = lzcnt (rev (w2bits w1)) then 0 else 2 ^ (32 - lzcnt (rev (w2bits w1)) - 1)) <
+proof.
+  rewrite W32.to_uintE /leak_div.
+  have := lzcnt_bound (w2bits w1).
+  have := lzcnt_bound (w2bits w2).
+  rewrite !size_w2bits => h1 h2 h3.
+  have : (if 32 = lzcnt (rev (w2bits w1)) then 0 else 2 ^ (32 - lzcnt (rev (w2bits w1)) - 1)) <
       2 ^ (32 - lzcnt (rev (w2bits w2))) by smt().
-    case (32 = lzcnt (rev (w2bits w1))) => /= [ <- | ] h; 1: smt (leak_div_bound).
-      rewrite -ltr_weexpn2l 1://; smt(leak_div_bound).
-  qed.
+  case (32 = lzcnt (rev (w2bits w1))) => /= [ <- | ] h; 1: smt (leak_div_bound).
+  rewrite -ltr_weexpn2l 1://; smt(leak_div_bound).
+qed.
 
-(* Remark: the shift by 23 look arbitrary. I think a shift by 8 is suffisant *)
+(* Remark: the shift by 23 look arbitrary, a shift by 8 is suffisant *)
 lemma l_rotate_offset_div_core (x md_size : W32.t) :
   0 <= to_uint x < 2^8 =>
   16 <= to_uint md_size <= 64 =>
@@ -95,16 +106,16 @@ proof.
     rewrite !W32.get_to_uint hi /=.
     case: (i < 8) => hi'.
     + rewrite /md23 /(`<<`) /= W32.to_uint_shl 1:// IntDiv.modz_pow2_div.
-      + by apply StdOrder.IntOrder.divr_ge0; 1: smt(W32.to_uint_cmp).
+      + by apply divr_ge0; 1: smt(W32.to_uint_cmp).
       + smt().
       have h21 : 2 = 2 ^ 1 by done.
       rewrite {6}h21 modz_dvd_pow 1:/#.
       have -> : 2 ^ 23 = 2 ^ (23 - i - 1) * 2 * 2 ^ i.
-      + by rewrite {3}h21 -!Ring.IntID.exprD_nneg 1,3,4:/# 1://; congr; ring.
+      + by rewrite {3}h21 -!exprD_nneg 1,3,4:/# 1://; congr; ring.
       rewrite -(mulzA (W32.to_uint _)) mulzK; 1: smt(gt0_pow2).
       by rewrite -mulzA modzMl.
     rewrite divz_small //.
-    by have /= /# :=StdOrder.IntOrder.ler_weexpn2l 2 _ 8 i.
+    by have /= /# := ler_weexpn2l 2 _ 8 i.
   rewrite leak_div_or.
   have : leak_div (W32.of_int 256) <= leak_div x.
   + by apply leak_div_le => /= /#.
